wip

src/Lean/Meta/Tactic/Simp/Main.lean
@@ -259,14 +259,32 @@ private partial def reduce (e : Expr) : SimpM Expr := withIncRecDepth do
 
 private partial def dsimp (e : Expr) : M Expr := do
   let cfg ← getConfig
+  trace[Debug.Meta.Tactic.simp] "dsimp({e}, cfg.dsimp={cfg.dsimp})"
   unless cfg.dsimp do
     return e
+  let ctx ← readThe Simp.Context
   let pre (e : Expr) : M TransformStep := do
+    trace[Debug.Meta.Tactic.simp] "pre({e}), isOfNatNatLit=({isOfNatNatLit e})"
     if let Step.visit r ← rewritePre e (fun _ => pure none) (rflOnly := true) then
       if r.expr != e then
         return .visit r.expr
+    -- Block recursion into `OfNat.ofNat` literals
+    -- TODO: Don't we want to simplify the implicit type argument still?
+    if isOfNatNatLit e then
+      trace[Debug.Meta.Tactic.simp] "isOfNatNatLit!!!"
+      -- Recall that we expand "orphan" kernel nat literals `n` into `ofNat n`
+      return .done e
     return .continue
   let post (e : Expr) : M TransformStep := do
+    trace[Debug.Meta.Tactic.simp] "post({e})"
+    -- Normalize unenclosed `nat_lit n` into `OfNat.ofNat (nat_lit n)`
+    if let some n := e.natLit? then
+      trace[Debug.Meta.Tactic.simp] "is natLit? !!!"
+      /- If `OfNat.ofNat` is marked to be unfolded, we do not pack orphan nat literals as `OfNat.ofNat` applications
+         to avoid non-termination. See issue #788.  -/
+      if ¬ctx.isDeclToUnfold ``OfNat.ofNat then
+        return .visit (mkNatLit n)
+    -- fixme
     if let Step.visit r ← rewritePost e (fun _ => pure none) (rflOnly := true) then
       if r.expr != e then
         return .visit r.expr
@@ -390,7 +408,7 @@ where
       if (← readThe Simp.Context).isDeclToUnfold ``OfNat.ofNat then
         return { expr := e }
       else
-        return { expr := (← mkNumeral (mkConst ``Nat) n) }
+        return { expr := mkNatLit n }
     | none   => return { expr := e }
 
   simpProj (e : Expr) : M Result := do
